Move local to cfHeaps

characteristic/cfHeapsScript.sml
@@ -241,4 +241,64 @@ val hsimpl_gc = store_thm ("hsimpl_gc",
   fs [GC_def, SEP_IMP_def, SEP_EXISTS] \\ metis_tac []
 )
 
+(*------------------------------------------------------------------*)
+(** Locality *)
+
+(* local = frame rule + consequence rule + garbage collection *)
+
+val local_def = Define `
+  local cf env (H: hprop) (Q: v -> hprop) =
+    !(h: heap). H h ==> ?H1 H2 Q1.
+      (H1 * H2) h /\
+      cf env H1 Q1 /\
+      (Q1 *+ H2 ==+> Q *+ GC)`
+
+val is_local_def = Define `
+  is_local cf = (cf = local cf)`
+
+(* Properties of [local] *)
+
+val local_elim = store_thm ("local_elim",
+  ``!cf env H Q. cf env H Q ==> local cf env H Q``,
+  fs [local_def] \\ rpt strip_tac \\
+  Q.LIST_EXISTS_TAC [`H`, `emp`, `Q`] \\
+  rew_heap \\ fs [SEP_IMP_def, STAR_def] \\
+  rpt strip_tac \\ qcase_tac `Q x s` \\ Q.LIST_EXISTS_TAC [`{}`, `s`] \\
+  fs [GC_def, SEP_EXISTS] \\ strip_tac THEN1 SPLIT_TAC \\
+  qexists_tac `emp` \\ fs [emp_def]
+)
+
+val local_local = store_thm ("local_local",
+  ``!cf. local (local cf) = local cf``,
+  qsuff_tac `!cf env H Q. local (local cf) env H Q = local cf env H Q`
+  THEN1 (metis_tac []) \\
+  rpt strip_tac \\ eq_tac \\
+  fs [local_elim] \\
+  fs [local_def] \\ rpt strip_tac \\ first_x_assum drule \\
+  disch_then (qx_choosel_then [`H1`, `H2`, `Q1`] strip_assume_tac) \\
+  fs [STAR_def] \\ qcase_tac `SPLIT h (h1, h2)` \\
+  first_x_assum drule \\
+  disch_then (qx_choosel_then [`H1'`, `H2'`, `Q1'`] strip_assume_tac) \\
+  Q.LIST_EXISTS_TAC [`H1'`, `H2' * H2`, `Q1'`] \\ fs [PULL_EXISTS] \\
+  qcase_tac `SPLIT h1 (h11, h12)` \\
+  `SPLIT h (h11, h12 UNION h2)` by SPLIT_TAC \\
+  `(H2' * H2) (h12 UNION h2)` by (fs [STAR_def] \\ SPLIT_TAC) \\
+  asm_exists_tac \\ fs [] \\
+  fs [SEP_IMPPOST_def, STARPOST_def] \\ qx_gen_tac `x` \\
+  rpt (first_x_assum (qspec_then `x` assume_tac)) \\
+  rewrite_tac [STAR_ASSOC] \\
+  match_mp_tac SEP_IMP_TRANS \\ qexists_tac `Q1 x * GC * H2` \\ strip_tac
+  THEN1 (match_mp_tac SEP_IMP_STAR \\ fs [SEP_IMP_REFL]) \\
+  match_mp_tac SEP_IMP_TRANS \\ qexists_tac `Q x * (GC * GC)` \\ strip_tac
+  THENL [all_tac, fs [GC_STAR_GC, SEP_IMP_REFL]] \\
+  qsuff_tac `SEP_IMP ((Q1 x * H2) * GC) ((Q x * GC) * GC)`
+  THEN1 fs [AC STAR_ASSOC STAR_COMM] \\
+  match_mp_tac SEP_IMP_STAR \\ fs [SEP_IMP_REFL]
+)
+
+val local_is_local = store_thm ("local_is_local",
+  ``!F. is_local (local F) = T``,
+  metis_tac [is_local_def, local_local]
+)
+
 val _ = export_theory()
